spanning.v
@@ -56,109 +56,109 @@ which we are binding. *)
 Section Helpers.
   Context {Σ} {Ih : heapG Σ} {Im : markingG Σ} {Ig : graphG Σ} {Ii : invtokG Σ}.
 
-  Lemma wp_try_mark g Mrk k q (x : loc) w :
+  Lemma wp_try_mark g Mrk k q (x : loc) :
+    x ∈ dom (gset _) g →
     marked g = ∅ →
-    (heap_ctx ★ graph_ctx g Mrk ★ Γρ(q, x [↦] w) ★ κ(k))
+    (heap_ctx ★ graph_ctx g Mrk ★ Γρ(q, ∅) ★ κ(k))
       ⊢
       WP (try_mark #x)
       {{ v,
-         match v with
-         | # true =>
-           (∃ u, (w = None)
-                   ★ ((g !! x) = Some (false, u)) ★
-                   Γρ(q, x [↦] Excl' u))
-         | # false => Γρ(q, x [↦] w)
-         | _ => False
-         end
-           ★ μ(x) ★ κ(k)
+         (v = #true ★
+               (∃ u, ((g !! x) = Some (false, u))
+                       ★ Γρ(q, x [↦] u)) ★ μ(x) ★ κ(k))
+           ∨ (v = #false ★ Γρ(q, ∅) ★ μ(x) ★ κ(k))
       }}.
   Proof.
-    intros Hgnm. iIntros "(#Hheap & #Hgr & Hx & key)". unfold try_mark.
+    iIntros (Hgx Hgnm) "(#Hheap & #Hgr & Hx & key)". unfold try_mark.
     wp_let; wp_focus (! _)%E. unfold graph_ctx; iInv graphN as "Hinv".
-    open_graph_inv "Hinv" "key" γ mr "(Hi1 & Hi2 & Hi3 & Hi4 & Hi5)".
-    iDestruct (graph_open_later with "[Hx Hi1 Hi3 Hi5]") as
-        "(Hi1 & Hi3 & Hi5 & Hi6 & Hx)"; [by iFrame|].
-    rewrite later_exist. iDestruct "Hi6" as (u) "[Hi61 Hi62]".
-    rewrite later_exist. iDestruct "Hi62" as (m) "[Hi62 [Hi63 Hi64]]".
-    wp_load; iPvsIntro. iDestruct "Hi61" as %Hi61. iDestruct "Hi4" as %Hi4.
-    iDestruct "Hi1" as %Hi1. iDestruct "Hi62" as %Hi62.
-    iDestruct (graph_close with "[Hi3 Hi5 Hi63 Hi64 Hx]") as "(Hi1&Hi3&Hx)";
+    open_graph_inv "Hinv" "key" γ mr "(Hi1 & Hi2 & Hi3 & Hi4 & Hi5 & Hi6)".
+    iDestruct (@graph_open_later with "[Hi1 Hi3]") as
+        "(Hi1 & Hi3 & Hil)"; eauto; [by iFrame|].
+    rewrite later_exist. iDestruct "Hil" as (u) "[Hil1 Hil2]".
+    rewrite later_exist. iDestruct "Hil2" as (m) "[Hil2 [Hil3 Hil4]]".
+    wp_load; iPvsIntro. iDestruct "Hil1" as %Hil1. iDestruct "Hil2" as %Hil2.
+    iDestruct (graph_close with "[Hi3 Hil3 Hil4]") as "Hi3";
       eauto. iFrame. iExists _; eauto. iSplitR; eauto. by iExists _; iFrame.
-    iSplitL "Hi1 Hi2 Hi3".
-    { iNext. iApply Pack. iExists _, _; iFrame. by iSplitL; iPureIntro. }
+    iSplitL "Hi1 Hi2 Hi3 Hi5 Hi6 Hi4".
+    { iNext. iApply Pack. iExists _, _; iFrame; auto. }
     destruct u as [bu lu]; simpl. wp_focus (Fst _). iApply wp_fst; eauto.
     { by destruct lu as [[] []]; simpl; eauto. }
     iNext; iPvsIntro; wp_let. iInv graphN as "Hinv".
-    clear Hi4 Hi1 Hi61.
-    open_graph_inv "Hinv" "key" γ' mr' "(Hi1 & Hi2 & Hi3 & Hi4 & Hi5)".
-    iDestruct (graph_open_later with "[Hx Hi1 Hi3 Hi5]") as
-        "(Hi1 & Hi3 & Hi5 & Hi6 & Hx)"; [by iFrame|].
-    rewrite later_exist. iDestruct "Hi6" as (u) "[Hi61 Hi62]".
-    rewrite later_exist. iDestruct "Hi62" as (m') "[Hi62 [Hi63 Hi64]]".
-    iTimeless "Hi62". iDestruct "Hi62" as %Hi62'. rewrite Hi62' in Hi62.
-    iTimeless "Hi61". iDestruct "Hi61" as %Hi61.
+    open_graph_inv "Hinv" "key" γ' mr' "(Hi1 & Hi2 & Hi3 & Hi4 & Hi5 & Hi6)".
+    iDestruct (graph_open_later with "[Hi1 Hi3]") as
+        "(Hi1 & Hi3 & Hil)"; eauto; [by iFrame|].
+    rewrite later_exist. iDestruct "Hil" as (u) "[Hil1 Hil2]".
+    rewrite later_exist. iDestruct "Hil2" as (m') "[Hil2 [Hil3 Hil4]]".
+    iTimeless "Hil2". iDestruct "Hil2" as %Hil2'.
+    iTimeless "Hil1". iDestruct "Hil1" as %Hil1'.
+    iTimeless "Hi5". iDestruct "Hi5" as %Hi5.
+    iTimeless "Hi6". iDestruct "Hi6" as %Hi6.
     iTimeless "Hi4". iDestruct "Hi4" as %Hi4.
-    iTimeless "Hi1". iDestruct "Hi1" as %Hi1.
-    inversion Hi62; subst; clear Hi62.
+    rewrite Hil2' in Hil2; inversion Hil2; subst.
     destruct u as [[] lu']; simpl in *.
     - (* CAS fails *)
       wp_cas_fail.
-      iDestruct (graph_close with "[Hi3 Hi5 Hi63 Hi64 Hx]") as "(Hi1&Hi3&Hx)";
-      eauto. iFrame. iExists _; eauto. iSplitR; eauto. by iExists _; iFrame.
+      iDestruct (graph_close with "[Hi3 Hil3 Hil4]") as "Hi3";
+        eauto. iFrame. iExists _; eauto. iSplitR; eauto. by iExists _; iFrame.
       iPvs (already_marked with "Hi2") as "[Hi2 Hxm]"; [|iFrame "Hxm"].
       { rewrite Hi4. eapply graph.is_marked; eauto. }
-      iPvsIntro; iFrame. iNext; iApply Pack.
-      unfold graph_inv; iExists _, _; iFrame; by repeat iSplitL.
+      iPvsIntro; iFrame. iSplitR "Hx".
+      + iNext; iApply Pack.
+        unfold graph_inv; iExists _, _; iFrame; repeat iSplitL; trivial.
+      + by iRight; iFrame.
     - (* CAS succeeds *)
-      wp_cas_suc. rewrite (graph_expose_node g γ' x (false, lu')) //=.
-      iDestruct (graph_pointsto_unmarked with "[Hi3 Hx]")
-        as "[Hi3 [Hx %]]"; try by iFrame. by rewrite lookup_delete.
-      subst.
-      iPvs (mark_update_graph _ _ _ (Excl lu') with "[Hi3 Hx]") as "[Hi3 Hx]";
-        try by iFrame. done. by rewrite lookup_delete.
+      wp_cas_suc.
+      iDestruct (auth_own_graph_valid with "Hi1") as "[Hi1 H]".
+      iDestruct "H" as %Hv1.
+      iPvs (mark_graph _ _ x lu' with "[Hi1 Hx]") as "[Hi1 Hx]";
+        try by iFrame. eapply unmarked_in_graph_mon; eauto.
       iPvs (new_marked with "Hi2") as "[Hi2 Hm]". iFrame "key Hm".
-      erewrite mark_update_deleted.
-      iDestruct (graph_close with "[Hi3 Hi5 Hi63 Hi64 Hx]") as "(Hi1&Hi3&Hx)";
-        try iFrame.
-      { erewrite mark_update_dom_stable; eauto. }
-      { iExists (_, _). iSplitR; [| iExists _; by iFrame].
+      erewrite delete_marked.
+      iDestruct (auth_own_graph_valid with "Hi1") as "[Hi1 %]".
+      iDestruct (graph_close with "[Hi3 Hil3 Hil4]") as "Hi3".
+      { iFrame. iExists (_, _). iSplitR; [| iExists _; by iFrame].
           by rewrite mark_update_lookup. }
+      pose proof (unmarked_from_g _ _ _ _ Hv1 Hil1') as Hfg.
       iPvsIntro. iSplitR "Hx".
       + iNext; iApply Pack; unfold graph_inv. iExists _, _; iFrame.
-        iSplit; iPureIntro.
-        { by rewrite new_marking_dom marking_union Hi4. }
-        { erewrite mark_update_dom_stable; eauto. }
-      + iExists _; iFrame. iSplit; iPureIntro; eauto using unmarked_from_g.
+        repeat iSplit; iPureIntro.
+        { by rewrite new_marking_dom marking_union //= Hi4. }
+        { erewrite mark_dom_union => i. rewrite elem_of_union elem_of_singleton.
+          intros [?|?]; subst; auto. }
+        { apply agrees_op; trivial; split; eauto using nodes_agree_refl. }
+      + iLeft; iSplit; trivial. iExists _; by iFrame.
   Qed.
 
   Lemma wp_unmark_fst g Mrk k q (x : loc) w1 w2 :
+    (g !! x) = Some (false, (w1, w2)) →
     marked g = ∅ →
-    (heap_ctx ★ graph_ctx g Mrk ★ Γρ(q, x [↦] Excl' (w1, w2)) ★ κ(k))
+    (heap_ctx ★ graph_ctx g Mrk ★ Γρ(q, x [↦] (w1, w2)) ★ κ(k))
       ⊢
       WP (unmark_fst #x)
-      {{ _, Γρ(q, x [↦] Excl' (None, w2)) ★ κ(k) }}.
+      {{ _, Γρ(q, x [↦] (None, w2)) ★ κ(k) }}.
   Proof.
-    intros Hgnm. iIntros "(#Hheap & #Hgr & Hx & key)". unfold unmark_fst.
+    iIntros (Hgx Hgnm) "(#Hheap & #Hgr & Hx & key)". unfold unmark_fst.
+    assert (Hgx' : x ∈ dom (gset _) g).
+    { rewrite elem_of_dom Hgx; eauto. }
     wp_let; wp_focus (! _)%E. unfold graph_ctx; iInv graphN as "Hinv".
-    open_graph_inv "Hinv" "key" γ mr "(Hi1 & Hi2 & Hi3 & Hi4 & Hi5)".
-    iDestruct (graph_open_later with "[Hx Hi1 Hi3 Hi5]") as
-        "(Hi1 & Hi3 & Hi5 & Hi6 & Hx)"; [by iFrame|].
-    rewrite later_exist. iDestruct "Hi6" as (u) "[Hi61 Hi62]".
-    rewrite later_exist. iDestruct "Hi62" as (m) "[Hi62 [Hi63 Hi64]]".
-    wp_load. iDestruct "Hi1" as %Hi1. iDestruct "Hi61" as %Hi61.
-    iDestruct "Hi62" as %Hi62. rewrite (graph_expose_node g γ x u) //=.
-    iDestruct (graph_pointsto_marked with "[Hi3 Hx]")
-      as "[Hi3 [Hx Heq]]"; try by iFrame. by rewrite lookup_delete.
-    iDestruct "Heq" as %Heq; rewrite Heq.
-    rewrite -> (graph_mon_to_ND _ _ Heq) in *. iPvsIntro.
-    iDestruct (graph_close with "[Hi3 Hi5 Hi63 Hi64 Hx]") as "(Hi1&Hi3&Hx)";
-      [|iFrame|].
-    { erewrite mark_update_dom_stable; eauto. }
-    { iExists _; eauto. iSplitR; [|by iExists _; iFrame].
-        by rewrite mark_update_lookup. }
-    iSplitL "Hi1 Hi2 Hi3 Hi4".
-    { iNext. iApply Pack. iExists _, _; iFrame.
-      erewrite mark_update_dom_stable; eauto. }
+    open_graph_inv "Hinv" "key" γ mr "(Hi1 & Hi2 & Hi3 & Hi4 & Hi5 & Hi6)".
+    iDestruct (graph_open_later with "[Hi1 Hi3]")
+      as "(Hi1 & Hi3 & Hil)"; eauto; [by iFrame|].
+    rewrite later_exist. iDestruct "Hil" as (u) "[Hil1 Hil2]".
+    rewrite later_exist. iDestruct "Hil2" as (m) "[Hil2 [Hil3 Hil4]]".
+    wp_load. iDestruct "Hi5" as %Hi5. iDestruct "Hil1" as %Hil1.
+    iDestruct "Hil2" as %Hil2. iDestruct "Hi6" as %Hi6. iDestruct "Hi4" as %Hi4.
+    iDestruct (auth_own_graph_valid with "Hi1") as "[Hi1 Hvγ]".
+    iDestruct "Hvγ" as %Hvγ. iDestruct (graph_pointsto_marked with "[Hi1 Hx]")
+      as "(Hi1 & Hx & Heq)"; try by iFrame.
+    pose proof Hil1 as Hil1'. iDestruct "Heq" as %Heq; rewrite Heq in Hil1' Hvγ.
+    rewrite mark_update_lookup in Hil1'; trivial.
+    iDestruct (graph_close with "[Hi3 Hil3 Hil4]") as "Hi3"; [iFrame|].
+    { iExists _; iSplitR; auto. iExists _; by iFrame. }
+    iPvsIntro. iSplitL "Hi1 Hi2 Hi3".
+    { iNext; iApply Pack. unfold graph_inv at 2.
+      iExists _, _; iFrame; repeat iSplit; by iPureIntro. }
+    clear Hil1 Hi6 Hi4 Hi5 Heq Hvγ. inversion Hil1'; subst. clear Hil1'.
     wp_let. wp_focus (Fst _). iApply wp_fst; eauto.
     { rewrite to_val_pr_opl_heap'; eauto. }
     iNext; iPvsIntro. wp_focus (Snd (_, _)). iApply wp_snd; eauto.
@@ -167,104 +167,155 @@ Section Helpers.
     { rewrite to_val_opl_heap; eauto. }
     {by rewrite to_val_opl_heap. }
     iNext; iPvsIntro.
-    iInv graphN as "Hinv". clear Hi1 Hi61 Heq u.
-    open_graph_inv "Hinv" "key" γ' mr' "(Hi1 & Hi2 & Hi3 & Hi4 & Hi5)".
-    iDestruct (graph_open_later with "[Hx Hi1 Hi3 Hi5]") as
-        "(Hi1 & Hi3 & Hi5 & Hi6 & Hx)"; [by iFrame|].
-    rewrite later_exist. iDestruct "Hi6" as (u) "[Hi61 Hi62]".
-    rewrite later_exist. iDestruct "Hi62" as (m') "[Hi62 [Hi63 Hi64]]".
-    iTimeless "Hi62". iDestruct "Hi62" as %Hi62'. rewrite Hi62' in Hi62.
-    iTimeless "Hi61". iDestruct "Hi61" as %Hi61.
-    iTimeless "Hi4". iDestruct "Hi4" as %Hi4.
-    iTimeless "Hi1". iDestruct "Hi1" as %Hi1.
-    inversion Hi62; subst; clear Hi62.
-    rewrite (graph_expose_node g γ' x u Hgnm Hi61). wp_store.
-    iDestruct (graph_pointsto_marked with "[Hi3 Hx]")
-      as "[Hi3 [Hx Heq]]"; try by iFrame. by rewrite lookup_delete.
-    iDestruct "Heq" as %Heq; rewrite Heq.
-    iPvs (mark_update_graph _ _ _ (Excl (None, w2)) with "[Hi3 Hx]") as
-        "[Hi3 Hx]"; try by iFrame. done. by rewrite lookup_delete.
-    rewrite -> (graph_mon_to_ND _ _ Heq) in *; simpl.
-    erewrite mark_update_deleted.
-    iDestruct (graph_close with "[Hi3 Hi5 Hi63 Hi64 Hx]") as "(Hi1&Hi3&Hx)";
-      try iFrame; simpl.
-      { erewrite mark_update_dom_stable; eauto. }
-      { rewrite mark_update_lookup.
-        iExists _. iSplitR; [eauto| iExists _; by iFrame]. }
-      iPvsIntro.
-      iNext; iApply Pack; unfold graph_inv. iExists _, _; iFrame.
-        iSplit; iPureIntro.
-        { rewrite -> (graph_expose_node g γ' x _ Hgnm Hi61) in Hi4.
-          by revert Hi4; rewrite ?marking_union. }
-        { erewrite mark_update_dom_stable; eauto. }
+    iInv graphN as "Hinv".
+    open_graph_inv "Hinv" "key" γ' mr' "(Hi1 & Hi2 & Hi3 & Hi4 & Hi5 & Hi6)".
+    iDestruct (graph_open_later with "[Hi1 Hi3]")
+      as "(Hi1 & Hi3 & Hil)"; eauto; [by iFrame|].
+    rewrite later_exist. iDestruct "Hil" as (u) "[Hil1 Hil2]".
+    rewrite later_exist. iDestruct "Hil2" as (m') "[Hil2 [Hil3 Hil4]]".
+    wp_store.
+    iDestruct "Hil2" as %Hil2'.
+    rewrite Hil2' in Hil2. inversion Hil2; subst; clear Hil2.
+    iDestruct "Hil1" as %Hil1. iDestruct "Hi4" as %Hi4. iDestruct "Hi5" as %Hi5.
+    iDestruct "Hi6" as %Hi6.
+    iDestruct (auth_own_graph_valid with "Hi1") as "[Hi1 Hvγ]".
+    iDestruct "Hvγ" as %Hvγ. iDestruct (graph_pointsto_marked with "[Hi1 Hx]")
+      as "(Hi1 & Hx & Heq)"; try by iFrame.
+    pose proof Hil1 as Hil1'. iDestruct "Heq" as %Heq; rewrite Heq in Hil1' Hvγ.
+    rewrite mark_update_lookup in Hil1'; trivial. inversion Hil1'; subst u.
+    clear Hil1'. simpl. rewrite Heq.
+    iPvs (update_graph _ _ _ (None, w2) with "[Hi1 Hx]") as
+        "[Hi1 Hx]"; try by iFrame. by rewrite lookup_delete.
+    rewrite -delete_marked. erewrite (delete_marked _ _ _ (None, w2)).
+    assert (Hvγ' : ✓ ({[x := Excl (None, w2)]} ⋅ delete x γ')).
+    { eapply updating_graph_valid; eauto. by rewrite lookup_delete. }
+    iDestruct (graph_close with "[Hi3 Hil3 Hil4]") as "Hi3".
+    { iFrame. iExists _. iSplitR.
+      - rewrite ?mark_update_lookup; eauto. - iExists _; by iFrame. }
+    iPvsIntro; iFrame.
+    iNext. iApply Pack. unfold graph_inv at 2.
+    iExists _, _; iFrame. repeat iSplit; iPureIntro.
+    { rewrite Heq in Hi4. rewrite Hi4 ?marking_union; trivial. }
+    { rewrite mark_dom_union => i.
+      rewrite elem_of_union dom_delete elem_of_singleton.
+      intros [->|Hdf]; trivial. apply elem_of_difference in Hdf.
+      apply Hi5; tauto. }
+    { apply agrees_op; trivial. split; [by apply agrees_deleted|].
+      eexists; split; eauto. destruct w2; done. }
   Qed.
 
   Lemma wp_unmark_snd g Mrk k q (x : loc) w1 w2 :
+    (g !! x) = Some (false, (w1, w2)) →
     marked g = ∅ →
-    (heap_ctx ★ graph_ctx g Mrk ★ Γρ(q, x [↦] Excl' (w1, w2)) ★ κ(k))
+    (heap_ctx ★ graph_ctx g Mrk ★ Γρ(q, x [↦] (w1, w2)) ★ κ(k))
       ⊢
       WP (unmark_snd #x)
-      {{ _, Γρ(q, x [↦] Excl' (w1, None)) ★ κ(k) }}.
+      {{ _, Γρ(q, x [↦] (w1, None)) ★ κ(k) }}.
   Proof.
-    intros Hgnm. iIntros "(#Hheap & #Hgr & Hx & key)". unfold unmark_snd.
+    iIntros (Hgx Hgnm) "(#Hheap & #Hgr & Hx & key)". unfold unmark_fst.
+    assert (Hgx' : x ∈ dom (gset _) g).
+    { rewrite elem_of_dom Hgx; eauto. }
     wp_let; wp_focus (! _)%E. unfold graph_ctx; iInv graphN as "Hinv".
-    open_graph_inv "Hinv" "key" γ mr "(Hi1 & Hi2 & Hi3 & Hi4 & Hi5)".
-    iDestruct (graph_open_later with "[Hx Hi1 Hi3 Hi5]") as
-        "(Hi1 & Hi3 & Hi5 & Hi6 & Hx)"; [by iFrame|].
-    rewrite later_exist. iDestruct "Hi6" as (u) "[Hi61 Hi62]".
-    rewrite later_exist. iDestruct "Hi62" as (m) "[Hi62 [Hi63 Hi64]]".
-    wp_load. iDestruct "Hi1" as %Hi1. iDestruct "Hi61" as %Hi61.
-    iDestruct "Hi62" as %Hi62. rewrite (graph_expose_node g γ x u) //=.
-    iDestruct (graph_pointsto_marked with "[Hi3 Hx]")
-      as "[Hi3 [Hx Heq]]"; try by iFrame. by rewrite lookup_delete.
-    iDestruct "Heq" as %Heq; rewrite Heq.
-    rewrite -> (graph_mon_to_ND _ _ Heq) in *. iPvsIntro.
-    iDestruct (graph_close with "[Hi3 Hi5 Hi63 Hi64 Hx]") as "(Hi1&Hi3&Hx)";
-      [|iFrame|].
-    { erewrite mark_update_dom_stable; eauto. }
-    { iExists _; eauto. iSplitR; [|by iExists _; iFrame].
-        by rewrite mark_update_lookup. }
-    iSplitL "Hi1 Hi2 Hi3 Hi4".
-    { iNext. iApply Pack. iExists _, _; iFrame.
-      erewrite mark_update_dom_stable; eauto. }
+    open_graph_inv "Hinv" "key" γ mr "(Hi1 & Hi2 & Hi3 & Hi4 & Hi5 & Hi6)".
+    iDestruct (graph_open_later with "[Hi1 Hi3]")
+      as "(Hi1 & Hi3 & Hil)"; eauto; [by iFrame|].
+    rewrite later_exist. iDestruct "Hil" as (u) "[Hil1 Hil2]".
+    rewrite later_exist. iDestruct "Hil2" as (m) "[Hil2 [Hil3 Hil4]]".
+    wp_load. iDestruct "Hi5" as %Hi5. iDestruct "Hil1" as %Hil1.
+    iDestruct "Hil2" as %Hil2. iDestruct "Hi6" as %Hi6. iDestruct "Hi4" as %Hi4.
+    iDestruct (auth_own_graph_valid with "Hi1") as "[Hi1 Hvγ]".
+    iDestruct "Hvγ" as %Hvγ. iDestruct (graph_pointsto_marked with "[Hi1 Hx]")
+      as "(Hi1 & Hx & Heq)"; try by iFrame.
+    pose proof Hil1 as Hil1'. iDestruct "Heq" as %Heq; rewrite Heq in Hil1' Hvγ.
+    rewrite mark_update_lookup in Hil1'; trivial.
+    iDestruct (graph_close with "[Hi3 Hil3 Hil4]") as "Hi3"; [iFrame|].
+    { iExists _; iSplitR; auto. iExists _; by iFrame. }
+    iPvsIntro. iSplitL "Hi1 Hi2 Hi3".
+    { iNext; iApply Pack. unfold graph_inv at 2.
+      iExists _, _; iFrame; repeat iSplit; by iPureIntro. }
+    clear Hil1 Hi6 Hi4 Hi5 Heq Hvγ. inversion Hil1'; subst. clear Hil1'.
     wp_let. wp_focus (Fst _). iApply wp_fst; eauto.
     { rewrite to_val_pr_opl_heap'; eauto. }
     iNext; iPvsIntro. wp_focus (Snd (_, _)). iApply wp_snd; eauto.
     { by rewrite to_val_pr_opl_heap'. }
     iNext; iPvsIntro. wp_focus (Fst _). iApply wp_fst; eauto.
-    { by rewrite to_val_opl_heap. }
+    {by rewrite to_val_opl_heap. }
     { rewrite to_val_opl_heap; eauto. }
     iNext; iPvsIntro.
-    iInv graphN as "Hinv". clear Hi1 Hi61 Heq u.
-    open_graph_inv "Hinv" "key" γ' mr' "(Hi1 & Hi2 & Hi3 & Hi4 & Hi5)".
-    iDestruct (graph_open_later with "[Hx Hi1 Hi3 Hi5]") as
-        "(Hi1 & Hi3 & Hi5 & Hi6 & Hx)"; [by iFrame|].
-    rewrite later_exist. iDestruct "Hi6" as (u) "[Hi61 Hi62]".
-    rewrite later_exist. iDestruct "Hi62" as (m') "[Hi62 [Hi63 Hi64]]".
-    iTimeless "Hi62". iDestruct "Hi62" as %Hi62'. rewrite Hi62' in Hi62.
-    iTimeless "Hi61". iDestruct "Hi61" as %Hi61.
-    iTimeless "Hi4". iDestruct "Hi4" as %Hi4.
-    iTimeless "Hi1". iDestruct "Hi1" as %Hi1.
-    inversion Hi62; subst; clear Hi62.
-    rewrite (graph_expose_node g γ' x u Hgnm Hi61). wp_store.
-    iDestruct (graph_pointsto_marked with "[Hi3 Hx]")
-      as "[Hi3 [Hx Heq]]"; try by iFrame. by rewrite lookup_delete.
-    iDestruct "Heq" as %Heq; rewrite Heq.
-    iPvs (mark_update_graph _ _ _ (Excl (w1, None)) with "[Hi3 Hx]") as
-        "[Hi3 Hx]"; try by iFrame. done. by rewrite lookup_delete.
-    rewrite -> (graph_mon_to_ND _ _ Heq) in *; simpl.
-    erewrite mark_update_deleted.
-    iDestruct (graph_close with "[Hi3 Hi5 Hi63 Hi64 Hx]") as "(Hi1&Hi3&Hx)";
-      try iFrame; simpl.
-      { erewrite mark_update_dom_stable; eauto. }
-      { rewrite mark_update_lookup.
-        iExists _. iSplitR; [eauto| iExists _; by iFrame]. }
-      iPvsIntro.
-      iNext; iApply Pack; unfold graph_inv. iExists _, _; iFrame.
-        iSplit; iPureIntro.
-        { rewrite -> (graph_expose_node g γ' x _ Hgnm Hi61) in Hi4.
-          by revert Hi4; rewrite ?marking_union. }
-        { erewrite mark_update_dom_stable; eauto. }
+    iInv graphN as "Hinv".
+    open_graph_inv "Hinv" "key" γ' mr' "(Hi1 & Hi2 & Hi3 & Hi4 & Hi5 & Hi6)".
+    iDestruct (graph_open_later with "[Hi1 Hi3]")
+      as "(Hi1 & Hi3 & Hil)"; eauto; [by iFrame|].
+    rewrite later_exist. iDestruct "Hil" as (u) "[Hil1 Hil2]".
+    rewrite later_exist. iDestruct "Hil2" as (m') "[Hil2 [Hil3 Hil4]]".
+    wp_store.
+    iDestruct "Hil2" as %Hil2'.
+    rewrite Hil2' in Hil2. inversion Hil2; subst; clear Hil2.
+    iDestruct "Hil1" as %Hil1. iDestruct "Hi4" as %Hi4. iDestruct "Hi5" as %Hi5.
+    iDestruct "Hi6" as %Hi6.
+    iDestruct (auth_own_graph_valid with "Hi1") as "[Hi1 Hvγ]".
+    iDestruct "Hvγ" as %Hvγ. iDestruct (graph_pointsto_marked with "[Hi1 Hx]")
+      as "(Hi1 & Hx & Heq)"; try by iFrame.
+    pose proof Hil1 as Hil1'. iDestruct "Heq" as %Heq; rewrite Heq in Hil1' Hvγ.
+    rewrite mark_update_lookup in Hil1'; trivial. inversion Hil1'; subst u.
+    clear Hil1'. simpl. rewrite Heq.
+    iPvs (update_graph _ _ _ (w1, None) with "[Hi1 Hx]") as
+        "[Hi1 Hx]"; try by iFrame. by rewrite lookup_delete.
+    rewrite -delete_marked. erewrite (delete_marked _ _ _ (w1, None)).
+    assert (Hvγ' : ✓ ({[x := Excl (w1, None)]} ⋅ delete x γ')).
+    { eapply updating_graph_valid; eauto. by rewrite lookup_delete. }
+    iDestruct (graph_close with "[Hi3 Hil3 Hil4]") as "Hi3".
+    { iFrame. iExists _. iSplitR.
+      - rewrite ?mark_update_lookup; eauto. - iExists _; by iFrame. }
+    iPvsIntro; iFrame.
+    iNext. iApply Pack. unfold graph_inv at 2.
+    iExists _, _; iFrame. repeat iSplit; iPureIntro.
+    { rewrite Heq in Hi4. rewrite Hi4 ?marking_union; trivial. }
+    { rewrite mark_dom_union => i.
+      rewrite elem_of_union dom_delete elem_of_singleton.
+      intros [->|Hdf]; trivial. apply elem_of_difference in Hdf.
+      apply Hi5; tauto. }
+    { apply agrees_op; trivial. split; [by apply agrees_deleted|].
+      eexists; split; eauto. destruct w1; done. }
   Qed.
+(*
+  Lemma rec_wp_span g Mrk k q (x : val) γ :
+    marked (of_base_graph g γ) = ∅ →
+    marked g = ∅ →
+    (x = NONEV ∨ ∃ l : loc, x = SOMEV #l ∧ l ∈ dom (gset positive) γ) →
+    (heap_ctx ★ graph_ctx g Mrk ★ Γρ(q, γ) ★ κ(k))
+      ⊢
+      WP (span x)
+      {{ v,
+         (v = # true ∧
+          ∃ l : loc,
+            x = SOMEV #l ∧
+            (∃ γ' (mmr : (maximal_marked_tree (of_base_graph g γ') l)),
+                Γρ(q, γ') ★
+                  ([★ set] l ∈
+                           (front
+                              (of_base_graph g γ')
+                              (marked (of_base_graph g γ'))) , μ(l))
+            ) ★ μ(l) ★ κ(k)
+          )
+         ∨
+         (v = # false ∧ x = NONEV ∧ Γρ(q, γ) ★ κ(k))
+      }}.
+  Proof.
+    intros Hunm Hgnm Hx. iIntros "(#Hheap & #Hgr & Hx & key)".
+    iRevert (q) "Hx". iLöb as "IH". iIntros (q) "Hx".
+    wp_rec. destruct Hx as [|[l [? Hlid]]]; subst.
+    { wp_match. iPvsIntro. iRight; repeat iSplit; trivial; by iFrame. }
+    wp_match. erewrite (own_graph_get_singleton _ _ _ l); eauto.
+*)
 
+
+
+
+
+
+
+
+    
+    
 End Helpers.
